proper names in fsub

dev2015/fsub0.v
@@ -38,21 +38,21 @@ Inductive tm : Type :=
   | tfalse : tm
   | tvar : id -> tm
   | tapp : tm -> tm -> tm (* f(x) *)
-  | tabs : tm -> tm (* \f x.y *)
+  | tabs : id -> id -> tm -> tm (* \f x.y *)
   | ttapp : tm -> ty -> tm (* f[X] *)
-  | ttabs : ty -> tm -> tm (* \f x.y *)
+  | ttabs : id -> ty -> tm -> tm (* \f x.y *)
 .
 
 Inductive vl : Type :=
-| vty   : list vl -> ty -> vl
-| vtya  : list vl -> ty -> vl (* X<T, only used in stp2_all *)
+| vty   : list (id*vl) -> ty -> vl
+| vtya  : list (id*vl) -> ty -> vl (* X<T, only used in stp2_all *)
 | vbool : bool -> vl
-| vabs  : list vl -> tm -> vl
-| vtabs : list vl -> ty -> tm -> vl
+| vabs  : list (id*vl) -> id -> id -> tm -> vl
+| vtabs : list (id*vl) -> id -> ty -> tm -> vl
 .
 
-Definition venv := list vl.
-Definition tenv := list ty.
+Definition venv := list (id*vl).
+Definition tenv := list (id*ty).
 
 Hint Unfold venv.
 Hint Unfold tenv.
@@ -63,20 +63,29 @@ Fixpoint length {X: Type} (l : list X): nat :=
     | _::l' => 1 + length l'
   end.
 
-Fixpoint index {X : Type} (n : id) (l : list X) : option X :=
+Fixpoint fresh {X: Type} (l : list (id * X)): nat :=
   match l with
-    | [] => None
-    | a :: l'  => if beq_nat n (length l') then Some a else index n l'
+    | [] => 0
+    | (n',a)::l' => 1 + n'
   end.
 
+Fixpoint index {X : Type} (n : id) (l : list (id * X)) : option X :=
+  match l with
+    | [] => None
+    | (n',a) :: l'  =>
+      if le_lt_dec (fresh l') n' then
+        if (beq_nat n n') then Some a else index n l'
+      else None
+  end.
+
+(*
 Fixpoint update {X : Type} (n : nat) (x: X)
                (l : list X) { struct l }: list X :=
   match l with
     | [] => []
-    (* for now, ignore binding value n' !!! *)
     | a :: l'  => if beq_nat n (length l') then x::l' else a :: update n x l'
   end.
-
+*)
 
 Inductive sub_env: tenv -> tenv -> Prop :=
 | se_refl: forall G,
@@ -186,7 +195,7 @@ Inductive stp: tenv -> ty -> ty -> Prop :=
     stp G1 (TSel x) (TSel x)
 | stp_all: forall G1 T1 T2 T3 T4,
     stp G1 T3 T1 ->
-    stp ((TMem T3)::G1) (open (TSel (length G1)) T2) (open (TSel (length G1)) T4) ->
+    stp ((fresh G1,TMem T3)::G1) (open (TSel (fresh G1)) T2) (open (TSel (fresh G1)) T4) ->
     stp G1 (TAll T1 T2) (TAll T3 T4)
 .
 (* TODO *)
@@ -203,9 +212,9 @@ Inductive has_type : tenv -> tm -> ty -> Prop :=
            has_type env f (TFun T1 T2) ->
            has_type env x T1 ->
            has_type env (tapp f x) T2
-| t_abs: forall env y T1 T2,
-           has_type (T1::(TFun T1 T2)::env) y T2 -> 
-           has_type env (tabs y) (TFun T1 T2)
+| t_abs: forall env f x y T1 T2,
+           has_type ((x,T1)::(f,TFun T1 T2)::env) y T2 -> 
+           has_type env (tabs f x y) (TFun T1 T2)
 | t_tapp: forall env f T11 T12 ,
            has_type env f (TAll T11 T12) ->
            has_type env (ttapp f T11) (open T11 T12)
@@ -219,9 +228,9 @@ Does it make a difference? It seems like we can always widen f?
            has_type env (ttapp f T2) (open T2 T12)
 
 *)                    
-| t_tabs: forall env y T1 T2,
-           (forall G2, sub_env env G2 -> has_type ((TMem T1)::G2) y (open (TSel (length G2)) T2)) -> 
-           has_type env (ttabs T1 y) (TAll T1 T2)
+| t_tabs: forall env x y T1 T2,
+           has_type ((x,TMem T1)::env) y (open (TSel x) T2) -> 
+           has_type env (ttabs x T1 y) (TAll T1 T2)
 (* TODO: subsumption *)
 .
 
@@ -263,8 +272,8 @@ Inductive stp2: venv -> ty -> venv -> ty -> Prop :=
 | stp2_all: forall G1 G2 T1 T2 T3 T4,
     stp2 G2 T3 G1 T1 ->
     (* watch out -- we put X<:T in the env, not X=T *)
-    stp2 ((vtya G2 T3)::G1) (open (TSel (length G1)) T2)
-         ((vtya G2 T3)::G2) (open (TSel (length G2)) T4) ->
+    stp2 ((fresh G1,vtya G2 T3)::G1) (open (TSel (fresh G1)) T2)
+         ((fresh G2,vtya G2 T3)::G2) (open (TSel (fresh G2)) T4) ->
     stp2 G1 (TAll T1 T2) G2 (TAll T3 T4)
 
 (*         
@@ -291,10 +300,10 @@ perhaps:
 
 Inductive wf_env : venv -> tenv -> Prop := 
 | wfe_nil : wf_env nil nil
-| wfe_cons : forall v t vs ts,
-    val_type (v::vs) v t ->
+| wfe_cons : forall n v t vs ts,
+    val_type ((n,v)::vs) v t ->
     wf_env vs ts ->
-    wf_env (cons v vs) (cons t ts)
+    wf_env (cons (n,v) vs) (cons (n,t) ts)
 
 with val_type : venv -> vl -> ty -> Prop :=
 | v_ty: forall env venv tenv T1 TE,
@@ -304,16 +313,16 @@ with val_type : venv -> vl -> ty -> Prop :=
 | v_bool: forall venv b TE,
     stp2 [] TBool venv TE ->
     val_type venv (vbool b) TE
-| v_abs: forall env venv tenv y T1 T2 TE,
+| v_abs: forall env venv tenv f x y T1 T2 TE,
     wf_env venv tenv ->
-    has_type (T1::(TFun T1 T2)::tenv) y T2 ->
+    has_type ((x,T1)::(f,TFun T1 T2)::tenv) y T2 ->
     stp2 venv (TFun T1 T2) env TE -> 
-    val_type env (vabs venv y) TE
-| v_tabs: forall env venv tenv y T1 T2 TE,
+    val_type env (vabs venv f x y) TE
+| v_tabs: forall env venv tenv x y T1 T2 TE,
     wf_env venv tenv ->
-    (forall G2, sub_env tenv G2 -> has_type ((TMem T1)::G2) y (open (TSel (length G2)) T2)) ->
+    has_type ((x,TMem T1)::tenv) y (open (TSel x) T2) ->
     stp2 venv (TAll T1 T2) env TE ->
-    val_type env (vtabs venv T1 y) TE
+    val_type env (vtabs venv x T1 y) TE
 .
 
 
@@ -335,8 +344,8 @@ Fixpoint teval(n: nat)(env: venv)(t: tm){struct n}: option (option vl) :=
         | ttrue      => Some (Some (vbool true))
         | tfalse     => Some (Some (vbool false))
         | tvar x     => Some (index x env)
-        | tabs y     => Some (Some (vabs env y))
-        | ttabs T y  => Some (Some (vtabs env T y))
+        | tabs f x y => Some (Some (vabs env f x y))
+        | ttabs x T y  => Some (Some (vtabs env x T y))
         | tapp ef ex   =>
           match teval n env ex with
             | None => None
@@ -348,9 +357,9 @@ Fixpoint teval(n: nat)(env: venv)(t: tm){struct n}: option (option vl) :=
                 | Some (Some (vbool _)) => Some None
                 | Some (Some (vty _ _)) => Some None
                 | Some (Some (vtya _ _)) => Some None
-                | Some (Some (vtabs _ _ _)) => Some None
-                | Some (Some (vabs env2 ey)) =>
-                  teval n (vx::(vabs env2 ey)::env2) ey
+                | Some (Some (vtabs _ _ _ _)) => Some None
+                | Some (Some (vabs env2 f x ey)) =>
+                  teval n ((x,vx)::(f,vabs env2 f x ey)::env2) ey
               end
           end
         | ttapp ef ex   =>
@@ -360,9 +369,9 @@ Fixpoint teval(n: nat)(env: venv)(t: tm){struct n}: option (option vl) :=
             | Some (Some (vbool _)) => Some None
             | Some (Some (vty _ _)) => Some None
             | Some (Some (vtya _ _)) => Some None
-            | Some (Some (vabs _ _)) => Some None
-            | Some (Some (vtabs env2 T ey)) =>
-              teval n ((vty env ex)::env2) ey
+            | Some (Some (vabs _ _ _ _)) => Some None
+            | Some (Some (vtabs env2 x T ey)) =>
+              teval n ((x,vty env ex)::env2) ey
           end
       end
   end.
@@ -386,69 +395,81 @@ Hint Unfold length.
 
 Hint Resolve ex_intro.
 
-Lemma wf_length : forall vs ts,
+Lemma wf_fresh : forall vs ts,
                     wf_env vs ts ->
-                    (length vs = length ts).
+                    (fresh vs = fresh ts).
 Proof.
   intros. induction H. auto.
-  assert ((length (v::vs)) = 1 + length vs). constructor.
-  assert ((length (t::ts)) = 1 + length ts). constructor.
-  rewrite IHwf_env in H1. auto.
-Qed.
-
-Hint Immediate wf_length.
-
-Lemma index_max : forall X vs n (T: X),
-                       index n vs = Some T ->
-                       n < length vs.
-Proof.
-  intros X vs. induction vs.
-  Case "nil". intros. inversion H.
-  Case "cons".
-  intros. inversion H.
-  case_eq (beq_nat n (length vs)); intros E.
-  SCase "hit".
-  rewrite E in H1. inversion H1. subst.
-  eapply beq_nat_true in E. 
-  unfold length. unfold length in E. rewrite E. eauto.
-  SCase "miss".
-  rewrite E in H1.
-  assert (n < length vs). eapply IHvs. apply H1.
   compute. eauto.
 Qed.
 
+Hint Immediate wf_fresh.
 
-
-
-
-Lemma index_extend : forall X vs n a (T: X),
+Lemma index_max : forall X vs n (T: X),
                        index n vs = Some T ->
-                       index n (a::vs) = Some T.
+                       n < fresh vs.
+Proof.
+  intros X vs. induction vs.
+  - Case "nil". intros. inversion H.
+  - Case "cons".
+    intros. inversion H. destruct a.
+    case_eq (le_lt_dec (fresh vs) i); intros ? E1.
+    + SCase "ok".
+      rewrite E1 in H1.
+      case_eq (beq_nat n i); intros E2.
+      * SSCase "hit".
+        eapply beq_nat_true in E2. subst n. compute. eauto.
+      * SSCase "miss".
+        rewrite E2 in H1.
+        assert (n < fresh vs). eapply IHvs. apply H1.
+        compute. omega.
+    + SCase "bad".
+      rewrite E1 in H1. inversion H1.
+Qed.
+
+Lemma le_xx : forall a b,
+                       a <= b ->
+                       exists E, le_lt_dec a b = left E.
+Proof. intros.
+  case_eq (le_lt_dec a b). intros. eauto.
+  intros. omega.     
+Qed.
+
+Lemma index_extend : forall X vs n n' x (T: X),
+                       index n vs = Some T ->
+                       fresh vs <= n' ->
+                       index n ((n',x)::vs) = Some T.
 
 Proof.
   intros.
-  assert (n < length vs). eapply index_max. eauto.
-  assert (n <> length vs). omega.
-  assert (beq_nat n (length vs) = false) as E. eapply beq_nat_false_iff; eauto.
-  unfold index. unfold index in H. rewrite H. rewrite E. reflexivity.
+  assert (n < fresh vs). eapply index_max. eauto.
+  assert (n <> n'). omega.
+  assert (beq_nat n n' = false) as E. eapply beq_nat_false_iff; eauto.
+  assert (fresh vs <= n') as E2. omega.
+  elim (le_xx (fresh vs) n' E2). intros ? EX.
+  unfold index. unfold index in H. rewrite H. rewrite E. rewrite EX. reflexivity.
 Qed.
 
-Lemma stp_extend : forall v1 G1 T1 T2,
+
+Lemma stp_extend : forall x v1 G1 T1 T2,
                        stp G1 T1 T2 ->
-                       stp (v1::G1) T1 T2.
+                       fresh G1 <= x ->
+                       stp ((x,v1)::G1) T1 T2.
 Proof. intros. induction H; eauto.
        eapply stp_sel1. eapply index_extend; eauto.
 admit. (* TAll *)
 Qed.
 
-Lemma stp2_extend2 : forall v1 G1 G2 T1 T2,
+Lemma stp2_extend2 : forall x v1 G1 G2 T1 T2,
                        stp2 G1 T1 G2 T2 ->
-                       stp2 G1 T1 (v1::G2) T2.
+                       fresh G2 <= x ->
+                       stp2 G1 T1 ((x,v1)::G2) T2.
 Proof. admit. Qed.
 
-Lemma stp2_extend1 : forall v1 G1 G2 T1 T2,
+Lemma stp2_extend1 : forall x v1 G1 G2 T1 T2,
                        stp2 G1 T1 G2 T2 ->
-                       stp2 (v1::G1) T1 G2 T2.
+                       fresh G1 <= x ->
+                       stp2 ((x,v1)::G1) T1 G2 T2.
 Proof. admit. Qed.
 
 Lemma stp2_reg2 : forall G1 G2 T1 T2,
@@ -463,11 +484,13 @@ Proof. admit. Qed.
 
 
 
-Lemma valtp_extend : forall vs v v1 T,
+Lemma valtp_extend : forall vs v x v1 T,
                        val_type vs v T ->
-                       val_type (v1::vs) v T.
-Proof. intros. induction H; eauto; econstructor; eauto; eapply stp2_extend2; eauto.  Qed.
-
+                       fresh vs <= x ->
+                       val_type ((x,v1)::vs) v T.
+Proof.
+  intros. induction H; eauto; econstructor; eauto; eapply stp2_extend2; eauto.
+Qed.
 
 
 Lemma index_safe_ex: forall H1 G1 TF i,
@@ -475,23 +498,29 @@ Lemma index_safe_ex: forall H1 G1 TF i,
              index i G1 = Some TF ->
              exists v, index i H1 = Some v /\ val_type H1 v TF.
 Proof. intros. induction H.
-       Case "nil". inversion H0.
-       Case "cons". inversion H0.
-         case_eq (beq_nat i (length ts)).
-           SCase "hit".
-             intros E.
-             rewrite E in H3. inversion H3. subst t.
-             assert (beq_nat i (length vs) = true). eauto.
-             assert (index i (v :: vs) = Some v). eauto.  unfold index. rewrite H2. eauto.
-             eauto.
-           SCase "miss".
-             intros E.
-             assert (beq_nat i (length vs) = false). eauto.
-             rewrite E in H3.
-             assert (exists v0, index i vs = Some v0 /\ val_type vs v0 TF) as HI. eapply IHwf_env. eauto.
-           inversion HI as [v0 HI1]. inversion HI1. 
-           eexists. econstructor. eapply index_extend; eauto. eapply valtp_extend; eauto.
+   - Case "nil". inversion H0.
+   - Case "cons". inversion H0.
+     case_eq (le_lt_dec (fresh ts) n); intros ? E1.
+     + SCase "ok".
+       rewrite E1 in H3.
+       assert ((fresh ts) <= n) as QF. eauto. rewrite <-(wf_fresh vs ts H1) in QF.
+       elim (le_xx (fresh vs) n QF). intros ? EX.
+
+       case_eq (beq_nat i n); intros E2.
+       * SSCase "hit".         
+         assert (index i ((n, v) :: vs) = Some v). eauto. unfold index. rewrite EX. rewrite E2. eauto.
+         assert (t = TF).
+         unfold index in H0. rewrite E1 in H0. rewrite E2 in H0. inversion H0. eauto.
+         subst t. eauto.
+       * SSCase "miss".
+         rewrite E2 in H3.
+         assert (exists v0, index i vs = Some v0 /\ val_type vs v0 TF) as HI. eapply IHwf_env. eauto.
+         inversion HI as [v0 HI1]. inversion HI1.
+         eexists. econstructor. eapply index_extend; eauto. eapply valtp_extend; eauto.
+     + SSCase "bad".
+       rewrite E1 in H3. inversion H3.
 Qed.
+
 
   
 Inductive res_type: venv -> option vl -> ty -> Prop :=
@@ -513,25 +542,25 @@ Lemma stp2_trans: forall G1 G2 G3 T1 T2 T3,
 Proof. admit. Qed.
 
 (* used in trans -- need to generalize interface for induction *)
-Lemma stp2_narrow: forall G1 G2 G3 G4 T1 T2 T3 T4,
+Lemma stp2_narrow: forall x G1 G2 G3 G4 T1 T2 T3 T4,
   stp2 G1 T1 G2 T2 ->
-  stp2 ((vtya G2 T2)::G3) T3 ((vtya G2 T2)::G4) T4 ->
-  stp2 ((vtya G1 T1)::G3) T3 ((vtya G1 T1)::G4) T4.
+  stp2 ((x,vtya G2 T2)::G3) T3 ((x,vtya G2 T2)::G4) T4 ->
+  stp2 ((x,vtya G1 T1)::G3) T3 ((x,vtya G1 T1)::G4) T4.
 Proof. admit. Qed.
 
 (* used in inversion *)
-Lemma stp2_narrow_concrete: forall G2 G3 G4 T2 T3 T4,
-  stp2 ((vtya G2 T2)::G3) T3 ((vtya G2 T2)::G4) T4 ->
-  stp2 ((vty G2 T2)::G3) T3 ((vty G2 T2)::G4) T4.
+Lemma stp2_narrow_concrete: forall x G2 G3 G4 T2 T3 T4,
+  stp2 ((x,vtya G2 T2)::G3) T3 ((x,vtya G2 T2)::G4) T4 ->
+  stp2 ((x,vty G2 T2)::G3) T3 ((x,vty G2 T2)::G4) T4.
 Proof.
   admit.
   (* selx becomes sel1/sel2 *)
 Qed.
 
 (* stp_subst *)
-Lemma stp2_subst: forall G1 T1 G2 T2 TX,
-  stp2 G1 T1 (vty G2 TX :: G2) (open (TSel (length G2)) T2) ->
-  stp2 G1 T1 (vty G2 TX :: G2) (open TX T2).
+Lemma stp2_subst: forall x G1 T1 G2 T2 TX,
+  stp2 G1 T1 ((x,vty G2 TX) :: G2) (open (TSel (length G2)) T2) ->
+  stp2 G1 T1 ((x,vty G2 TX) :: G2) (open TX T2).
 Proof.
   admit.
 Qed.
@@ -569,46 +598,55 @@ Qed.
 
 Lemma invert_abs: forall venv vf T1 T2,
   val_type venv vf (TFun T1 T2) ->
-  exists env tenv y T3 T4,
-    vf = (vabs env y) /\ 
+  exists env tenv f x y T3 T4,
+    vf = (vabs env f x y) /\
+    fresh env <= f /\
+    1 + f <= x /\
     wf_env env tenv /\
-    has_type (T3::(TFun T3 T4)::tenv) y T4 /\
+    has_type ((x,T3)::(f,TFun T3 T4)::tenv) y T4 /\
     stp2 venv T1 env T3 /\
     stp2 env T4 venv T2.
 Proof.
   intros. inversion H; try solve by inversion. inversion H2. subst. repeat eexists; repeat eauto.
+  admit. (* fresh *)
+  admit.
 Qed.
 
 Lemma invert_tabs: forall venv vf T1 T2,
   val_type venv vf (TAll T1 T2) ->
-  exists env tenv y T3 T4,
-    vf = (vtabs env T3 y) /\ 
+  exists env tenv x y T3 T4,
+    vf = (vtabs env x T3 y) /\
+    fresh env <= x /\
     wf_env env tenv /\
-    has_type ((TMem T3)::tenv) y (open (TSel (length tenv)) T4) /\
+    has_type ((x,TMem T3)::tenv) y (open (TSel x) T4) /\
     stp2 venv T1 env T3 /\
-    stp2 ((vty venv T1)::env) (open (TSel (length tenv)) T4) venv (open T1 T2).
+    stp2 ((x,vty venv T1)::env) (open (TSel x) T4) venv (open T1 T2).
 Proof.
-  intros. inversion H; try solve by inversion. inversion H2. subst. repeat eexists; repeat eauto. eapply H1. eapply se_refl.
+  intros. inversion H; try solve by inversion. inversion H2. subst. repeat eexists; repeat eauto.
+  admit.
+  admit.
+  (*
+  remember fresh
   (* inversion of TAll < TAll *)
   assert (stp2 venv0 T1 venv1 T0). eauto.
-  assert (stp2 (vtya venv0 T1 :: venv1) (open (TSel (length venv1)) T3)
-               (vtya venv0 T1 :: venv0) (open (TSel (length venv0)) T2)). eauto.
+  assert (stp2 ((x,vtya venv0 T1) :: venv1) (open (TSel x) T3)
+               ((x,vtya venv0 T1) :: venv0) (open (TSel x) T2)). eauto.
 
   (* narrow vtya to vty: X<T to X=T *)
-  assert (stp2 (vty venv0 T1 :: venv1) (open (TSel (length venv1)) T3)
-               (vty venv0 T1 :: venv0) (open (TSel (length venv0)) T2)). eapply stp2_narrow_concrete. eauto.
+  assert (stp2 ((x,vty venv0 T1) :: venv1) (open (TSel x) T3)
+               ((x,vty venv0 T1) :: venv0) (open (TSel x) T2)). eapply stp2_narrow_concrete. eauto.
 
   (* substitute *)
-  assert (stp2 (vty venv0 T1 :: venv1) (open (TSel (length venv1)) T3)
-               (vty venv0 T1 :: venv0) (open T1 T2)).
+  assert (stp2 ((x,vty venv0 T1) :: venv1) (open (TSel x) T3)
+               ((x,vty venv0 T1) :: venv0) (open T1 T2)).
   eapply stp2_subst. eauto.
   
   (* smaller env -- ok because val_type venv vf (TAll T1 T2) *)
-  assert (stp2 (vty venv0 T1 :: venv1) (open (TSel (length venv1)) T3)
+  assert (stp2 ((x,vty venv0 T1) :: venv1) (open (TSel x) T3)
                venv0 (open T1 T2)). admit.
 
-  assert (length venv1 = length tenv0) as E. eauto.
-  rewrite <- E. eauto.
+  assert (fresh tenv0 = fresh venv1) as E. eapply wf_fresh.
+  rewrite <- E. eauto.*)
 Qed. 
 
 
@@ -646,22 +684,22 @@ Proof.
     inversion HRF as [? vf].
 
     destruct (invert_abs venv0 vf T1 T2) as
-        [env1 [tenv [y0 [T3 [T4 [EF [WF [HTY [STX STY]]]]]]]]]. eauto.
+        [env1 [tenv [f0 [x0 [y0 [T3 [T4 [EF [FRF [FRX [WF [HTY [STX STY]]]]]]]]]]]]]. eauto.
     (* now we know it's a closure, and we have has_type evidence *)
 
-    assert (res_type (vx::vf::env1) res T4) as HRY.
+    assert (res_type ((x0,vx)::(f0,vf)::env1) res T4) as HRY.
       SCase "HRY".
         subst. eapply IHn. eauto. eauto.
-        (* wf_env f x *) econstructor. eapply valtp_widen; eauto. eapply stp2_extend2. eapply stp2_extend2. eauto.
-        (* wf_env f   *) econstructor. eapply v_abs; eauto. eapply stp2_extend2. eapply stp2_fun. eapply stp2_reg2. eauto. eapply stp2_reg1. eauto.
+        (* wf_env f x *) econstructor. eapply valtp_widen; eauto. eapply stp2_extend2. eapply stp2_extend2. eauto. eauto. eauto. 
+        (* wf_env f   *) econstructor. eapply v_abs; eauto. eapply stp2_extend2. eapply stp2_fun. eapply stp2_reg2. eauto. eapply stp2_reg1. eauto. eauto.
         eauto. 
 
     inversion HRY as [? vy].
 
-    eapply not_stuck. eapply valtp_widen; eauto. eapply stp2_extend1. eapply stp2_extend1. eauto.
+    eapply not_stuck. eapply valtp_widen; eauto. eapply stp2_extend1. eapply stp2_extend1. eauto. eauto. eauto.
     
   Case "Abs". intros. inversion H. inversion H0.
-    subst. inversion H11. subst.
+    subst. inversion H12. subst.
     eapply not_stuck. eapply v_abs; eauto. admit. (* has_type_wf *)
 
   Case "TApp".
@@ -674,22 +712,22 @@ Proof.
 
     subst t.
     destruct (invert_tabs venv0 vf T11 T12) as
-        [env1 [tenv [y0 [T3 [T4 [EF [WF [HTY [STX STY]]]]]]]]]. eauto.
+        [env1 [tenv [x0 [y0 [T3 [T4 [EF [FRX [WF [HTY [STX STY]]]]]]]]]]]. eauto.
     (* now we know it's a closure, and we have has_type evidence *)
 
-    assert (res_type ((vty venv0 T11)::env1) res (open (TSel (length tenv)) T4)) as HRY.
+    assert (res_type ((x0,vty venv0 T11)::env1) res (open (TSel x0) T4)) as HRY.
       SCase "HRY".
         subst. eapply IHn. eauto. eauto.
         (* wf_env x *) econstructor. eapply v_ty. 
         (* wf_env   *) eauto.
-    eapply stp2_extend2. eapply stp2_mem. eauto.
+    eapply stp2_extend2. eapply stp2_mem. eauto. eauto.
     eauto.
     inversion HRY as [? vy].
 
     eapply not_stuck. eapply valtp_widen; eauto.
 
   Case "TAbs". intros. inversion H. inversion H0.
-    subst. inversion H11. subst.
+    subst. inversion H12. subst.
     eapply not_stuck. eapply v_tabs; eauto. admit. (* has_type_wf *)
     
 Qed.
